WIP

src/tls/krml_output/hacks.h
@@ -3,8 +3,12 @@
 typedef void *FStar_Char_char_, *CoreCrypto_hash_ctx, *CoreCrypto_cipher_stream,
   *Platform_Date_dateTime, *Platform_Date_timeSpan;
 
+typedef int FStar_Char;
+
 #define FStar_Seq_Base_length(x) 0
 #define FStar_Seq_Base_init(x, y) 0
 #define FStar_Seq_Properties_split(x, y) ((K___FStar_Seq_Base_seq_FStar_Char_char__FStar_Seq_Base_seq_FStar_Char_char_){ .fst = 0, .snd = 0 })
 
 FStar_UInt16_t FStar_UInt16_uint_to_t(Prims_nat x);
+FStar_UInt32_t FStar_UInt32_uint_to_t(Prims_nat x);
+FStar_Char FStar_Char_char_of_int(krml_checked_int_t);
