src/tls/TLSConstants.fst
@@ -13,6 +13,12 @@ module TLSConstants
 //NS, JP: TODO, this include should eventually move to TLSMem, when that module exists
 include FStar.HyperStack.All
 
+let type_of (#a : Type) (x : a) : Type = a
+
+(* Start Hacks *)
+// assume val empty_bytes : Platform.Bytes.lbytes 0
+(* End Hacks *)
+
 open FStar.Seq
 open Platform.Date
 open Platform.Bytes
@@ -24,8 +30,6 @@ module HH = FStar.HyperHeap
 module HS = FStar.HyperStack
 
 include Parse // carving out basic formatting code to break a dependency.
-
-
 
 (** Polarity for reading and writing *)
 type rw =
@@ -1159,13 +1163,29 @@ let cipherSuite_of_name =
   | TLS_ECDHE_PSK_WITH_CHACHA20_POLY1305_SHA256    -> CipherSuite Kex_PSK_ECDHE None (AEAD CHACHA20_POLY1305 SHA256)
   | TLS_DHE_PSK_WITH_CHACHA20_POLY1305_SHA256      -> CipherSuite Kex_PSK_DHE None (AEAD CHACHA20_POLY1305 SHA256)
 
+(** Remove This after port, just trying to see if we can push it through Kremlin - @JROESCH *)
+let rec tot_map_cipherSuiteName (f : cipherSuiteName -> Tot valid_cipher_suite) (xs : list cipherSuiteName) : valid_cipher_suites =
+match xs with
+| [] -> []
+| (x :: xs) -> f x :: tot_map_cipherSuiteName f xs
+
+let rec tot_map_cipherSuiteName_eq_List_Tot_map (f : cipherSuiteName -> Tot valid_cipher_suite) (xs : list cipherSuiteName) :
+  Lemma (tot_map_cipherSuiteName f xs == List.Tot.map f xs) =
+match xs with
+| [] -> ()
+| (x :: xs) ->
+  assert (f x == f x);
+  tot_map_cipherSuiteName_eq_List_Tot_map f xs
+
 (** Return valid ciphersuites according to a list of ciphersuite names *)
 val cipherSuites_of_nameList: l1:list cipherSuiteName
   -> Tot (l2:valid_cipher_suites{List.Tot.length l2 = List.Tot.length l1})
 let cipherSuites_of_nameList nameList =
   // REMARK: would trigger automatically if List.Tot.Properties is loaded
+  tot_map_cipherSuiteName_eq_List_Tot_map cipherSuite_of_name nameList;
   List.Tot.map_lemma cipherSuite_of_name nameList;
-  List.Tot.map cipherSuite_of_name nameList
+  tot_map_cipherSuiteName cipherSuite_of_name nameList
+  // This doesn't work: tot_map_cipherSuiteName' cipherSuite_of_name nameList
 
 (** Determine the name of a ciphersuite based on its construction *)
 let name_of_cipherSuite =
@@ -1246,7 +1266,7 @@ let name_of_cipherSuite =
 #set-options "--max_ifuel 5 --initial_ifuel 5 --max_fuel 1 --initial_fuel 1"
 
 (** Determine the names associated to a list of ciphersuite constructors *)
-val names_of_cipherSuites : cipherSuites -> Tot (result cipherSuiteNames)
+(* val names_of_cipherSuites : cipherSuites -> Tot (result cipherSuiteNames)
 let rec names_of_cipherSuites css =
   match css with
   | [] -> Correct []
@@ -1260,7 +1280,10 @@ let rec names_of_cipherSuites css =
         | Error(x,y)  -> Error(x,y)
         | Correct rem -> Correct (n::rem)
       end
-    end
+    end *)
+
+// RESTORE ABOVE CODE - JROESCH
+assume val names_of_cipherSuites : cipherSuites -> Tot (result cipherSuiteNames)
 
 // Note:
 // Migrated contentType to Content.fst (this is internal to TLS)
@@ -1390,10 +1413,15 @@ let rec parseDistinguishedNameList data res =
 	  else Error(AD_decode_error, perror __SOURCE_FILE__ __LINE__ "")
         end
 
+(* REMOVE @jroesch *)
+val mem_cipherSuite: cipherSuite -> list cipherSuite -> Tot bool
+let rec mem_cipherSuite x = function
+| [] -> false
+| hd::tl -> if hd = x then true else mem_cipherSuite x tl
+
 (** Determine if a ciphersuite list contains the SCSV ciphersuite *)
 let contains_TLS_EMPTY_RENEGOTIATION_INFO_SCSV (css: list cipherSuite) =
-  List.Tot.mem (SCSV (TLS_EMPTY_RENEGOTIATION_INFO_SCSV)) css
-
+  mem_cipherSuite (SCSV (TLS_EMPTY_RENEGOTIATION_INFO_SCSV)) css
 
 // TODO: move all the definitions below to a separate file / figure out whether
 // they belong here ?
