src/tls/Extracted.mk
@@ -117,13 +117,16 @@ CEXE_PATH=LD_LIBRARY_PATH=./
 endif
 endif
 
-KRML_FILES = $(wildcard *.fst)
+KRML_FILES = TLSInfo.fst # $(wildcard *.fst)
+# We should add back support for Platform.Bytes when we get the chance.
+DROP_MODULES = $(addprefix -drop ,MonotoneMap Platform.Bytes Curve25519)
 C_DRIVER = $(KRML_DIR)/main.c
 HACKS_HEADER = '"hacks.h"'
 
 kremlin:
-	FSTAR_HOME=$(FSTAR_HOME) $(KRML) $(KRML_INCLUDE_PATHS) $(KRML_FILES) $(C_DRIVER) -I concrete-flags -add-include $(HACKS_HEADER) -fnoanonymous-unions -tmpdir $(KRML_DIR) \
-		   -warn-error +9+11-7 -derror-summary
+	FSTAR_HOME=$(FSTAR_HOME) $(KRML) $(KRML_INCLUDE_PATHS) $(KRML_FILES) $(C_DRIVER) \
+	           $(DROP_MODULES) -I concrete-flags -add-include $(HACKS_HEADER) -fnoanonymous-unions \
+			   -tmpdir $(KRML_DIR) $(KRML_OPTS) -warn-error +9+11-7-6 -derror-summary -skip-compilation
 
 test: test.out mitls.exe cmitls.exe
 	# Unit tests from test/test_main.ml
